ArkLib/OracleReduction/LiftContext/Reduction.lean
@@ -321,7 +321,7 @@ theorem liftContext_runWithLog
 
 end Reduction
 
-variable [∀ i, SelectableType (pSpec.Challenge i)]
+variable [∀ i, SampleableType (pSpec.Challenge i)]
   {σ : Type} {init : ProbComp σ} {impl : QueryImpl oSpec (StateT σ ProbComp)}
   {outerRelIn : Set (OuterStmtIn × OuterWitIn)} {outerRelOut : Set (OuterStmtOut × OuterWitOut)}
   {innerRelIn : Set (InnerStmtIn × InnerWitIn)} {innerRelOut : Set (InnerStmtOut × InnerWitOut)}
