ArkLib/OracleReduction/ProtocolSpec/Basic.lean
@@ -280,15 +280,15 @@ instance : Unique (ProtocolSpec 0) where
 instance : ∀ i, VCVCompatible (Challenge !p[] i) :=
   fun ⟨i, h⟩ =>
     (Fin.elim0 i : (h' : !p[].dir i = .V_to_P) → VCVCompatible (!p[].Challenge ⟨i, h'⟩)) h
-instance : ∀ i, SelectableType (Challenge !p[] i) :=
+instance : ∀ i, SampleableType (Challenge !p[] i) :=
   fun ⟨i, h⟩ =>
-    (Fin.elim0 i : (h' : !p[].dir i = .V_to_P) → SelectableType (!p[].Challenge ⟨i, h'⟩)) h
+    (Fin.elim0 i : (h' : !p[].dir i = .V_to_P) → SampleableType (!p[].Challenge ⟨i, h'⟩)) h
 instance : ∀ i, OracleInterface (Message !p[] i) :=
   fun ⟨i, h⟩ =>
     (Fin.elim0 i : (h' : !p[].dir i = .P_to_V) → OracleInterface (!p[].Message ⟨i, h'⟩)) h
 
 instance : ∀ i, VCVCompatible ((default : ProtocolSpec 0).Challenge i) := fun ⟨i, _⟩ => Fin.elim0 i
-instance : ∀ i, SelectableType ((default : ProtocolSpec 0).Challenge i) := fun ⟨i, _⟩ => Fin.elim0 i
+instance : ∀ i, SampleableType ((default : ProtocolSpec 0).Challenge i) := fun ⟨i, _⟩ => Fin.elim0 i
 instance : ∀ i, OracleInterface ((default : ProtocolSpec 0).Message i) := fun ⟨i, _⟩ => Fin.elim0 i
 
 variable {Msg Chal : Type}
@@ -302,7 +302,7 @@ instance [inst : OracleInterface Msg] : ∀ i, OracleInterface (Message ⟨!v[.P
   | ⟨0, _⟩ => inst
 instance : ∀ i, VCVCompatible (Challenge ⟨!v[.P_to_V], !v[Msg]⟩ i)
   | ⟨0, h⟩ => nomatch h
-instance : ∀ i, SelectableType (Challenge ⟨!v[.P_to_V], !v[Msg]⟩ i)
+instance : ∀ i, SampleableType (Challenge ⟨!v[.P_to_V], !v[Msg]⟩ i)
   | ⟨0, h⟩ => nomatch h
 
 instance : IsEmpty (MessageIdx ⟨!v[.V_to_P], !v[Chal]⟩) :=
@@ -314,7 +314,7 @@ instance : ∀ i, OracleInterface (Message ⟨!v[.V_to_P], !v[Chal]⟩ i)
   | ⟨0, h⟩ => nomatch h
 instance [inst : VCVCompatible Chal] : ∀ i, VCVCompatible (Challenge ⟨!v[.V_to_P], !v[Chal]⟩ i)
   | ⟨0, _⟩ => inst
-instance [inst : SelectableType Chal] : ∀ i, SelectableType (Challenge ⟨!v[.V_to_P], !v[Chal]⟩ i)
+instance [inst : SampleableType Chal] : ∀ i, SampleableType (Challenge ⟨!v[.V_to_P], !v[Chal]⟩ i)
   | ⟨0, _⟩ => inst
 
 variable {pSpec : ProtocolSpec n}
@@ -669,9 +669,9 @@ def getChallenge (pSpec : ProtocolSpec n) (i : pSpec.ChallengeIdx) :
 /-- Define the query implementation for the verifier's challenge in terms of `ProbComp`.
 
 This is a randomness oracle: it simply calls the `selectElem` method inherited from the
-  `SelectableType` instance on the challenge types.
+  `SampleableType` instance on the challenge types.
 -/
-def challengeQueryImpl {pSpec : ProtocolSpec n} [∀ i, SelectableType (pSpec.Challenge i)] :
+def challengeQueryImpl {pSpec : ProtocolSpec n} [∀ i, SampleableType (pSpec.Challenge i)] :
     QueryImpl ([pSpec.Challenge]ₒ'challengeOracleInterface) ProbComp where
   impl | query i () => uniformOfFintype (pSpec.Challenge i)
 
@@ -735,7 +735,7 @@ instance {pSpec : ProtocolSpec n} {Statement : Type} [∀ i, VCVCompatible (pSpe
     challenge given messages up to that point) in terms of `ProbComp`.
 
   This is a randomness oracle: it simply calls the `selectElem` method inherited from the
-  `SelectableType` instance on the challenge types. We may then augment this with `withCaching` to
+  `SampleableType` instance on the challenge types. We may then augment this with `withCaching` to
   obtain a function-like implementation (caches and replays previous queries).
 
   For implementation with caching, we add `withCaching`.
@@ -745,7 +745,7 @@ instance {pSpec : ProtocolSpec n} {Statement : Type} [∀ i, VCVCompatible (pSpe
 -/
 @[reducible, inline, specialize, simp]
 def srChallengeQueryImpl {Statement : Type} {pSpec : ProtocolSpec n}
-    [∀ i, SelectableType (pSpec.Challenge i)] :
+    [∀ i, SampleableType (pSpec.Challenge i)] :
     QueryImpl (srChallengeOracle Statement pSpec) ProbComp where
   impl | query i _ => uniformOfFintype (pSpec.Challenge i)
 
@@ -755,7 +755,7 @@ def srChallengeQueryImpl {Statement : Type} {pSpec : ProtocolSpec n}
   TODO: upstream this as a more general construction in VCVio -/
 @[reducible, inline, specialize, simp]
 def srChallengeQueryImpl' {Statement : Type} {pSpec : ProtocolSpec n}
-    [∀ i, SelectableType (pSpec.Challenge i)] :
+    [∀ i, SampleableType (pSpec.Challenge i)] :
     QueryImpl (srChallengeOracle Statement pSpec)
       (StateT (srChallengeOracle Statement pSpec).FunctionType ProbComp)
     where
