ArkLib/OracleReduction/Security/Basic.lean
@@ -34,7 +34,7 @@ variable {ι : Type} {oSpec : OracleSpec ι}
   {WitIn : Type}
   {StmtOut : Type} {ιₛₒ : Type} {OStmtOut : ιₛₒ → Type} [Oₛₒ : ∀ i, OracleInterface (OStmtOut i)]
   {WitOut : Type}
-  {n : ℕ} {pSpec : ProtocolSpec n} [∀ i, SelectableType (pSpec.Challenge i)]
+  {n : ℕ} {pSpec : ProtocolSpec n} [∀ i, SampleableType (pSpec.Challenge i)]
   -- Note: `σ` may depend on the previous data, like `StmtIn`, `pSpec`, and so on
   {σ : Type} (init : ProbComp σ) (impl : QueryImpl oSpec (StateT σ ProbComp))
 
@@ -401,7 +401,7 @@ end OracleProtocol
 variable {Statement : Type} {ιₛ : Type} {OStatement : ιₛ → Type}
   [∀ i, OracleInterface (OStatement i)] {Witness : Type}
   {n : ℕ} {pSpec : ProtocolSpec n}
-  [∀ i, SelectableType (pSpec.Challenge i)]
+  [∀ i, SampleableType (pSpec.Challenge i)]
   [∀ i, OracleInterface (pSpec.Message i)]
 
 namespace Proof
