ArkLib/OracleReduction/Security/StateRestoration.lean
@@ -92,7 +92,7 @@ variable {oSpec : OracleSpec ι}
   {WitIn : Type}
   {StmtOut : Type} {ιₛₒ : Type} {OStmtOut : ιₛₒ → Type} [Oₛₒ : ∀ i, OracleInterface (OStmtOut i)]
   {WitOut : Type}
-  {n : ℕ} {pSpec : ProtocolSpec n} [∀ i, SelectableType (pSpec.Challenge i)]
+  {n : ℕ} {pSpec : ProtocolSpec n} [∀ i, SampleableType (pSpec.Challenge i)]
   [DecidableEq StmtIn] [∀ i, DecidableEq (pSpec.Message i)] [∀ i, DecidableEq (pSpec.Challenge i)]
   (init : ProbComp (srChallengeOracle StmtIn pSpec).FunctionType)
   (impl : QueryImpl oSpec (StateT (srChallengeOracle StmtIn pSpec).FunctionType ProbComp))
